theories/L3_flattenedApp/wNorm.v
@@ -79,15 +79,11 @@ Proof.
   try (solve [inversion H; reflexivity]).
   - inversion_Clear H0.
     + rewrite (H _ H4) in n0. elim n0. auto.
-    + rewrite (H _ H5). reflexivity.
   - inversion H0.
     + rewrite (H args'). reflexivity. assumption.
   - inversion_Clear H1.
     + rewrite (H _ H5) in n1. elim n1. auto.
     + rewrite (H _ H4) in n. elim n. auto. 
     + rewrite (H _ H4) in n0. elim n0. auto.
-    + apply f_equal2.
-      * apply H. assumption.
-      * apply H0. assumption.
   - inversion_Clear H1. rewrite (H _ H4). rewrite (H0 _ H6). reflexivity.
 Qed.
